pkg/kernel/coq/Syntax.v
@@ -1,0 +1,150 @@
+Require Import Common.
+
+Inductive named_node_data : Set :=
+  | Named_Node : 
+      reference (* reference *)
+      -> named_node_data
+
+with named_node : Set :=
+  | NN_Library : library -> named_node
+  | NN_Class : class -> named_node
+  | NN_Member : member -> named_node
+
+
+with reference : Set :=
+  | Reference : 
+      nat
+      -> reference
+
+with library : Set :=
+  | Library : 
+      named_node_data
+      -> list class (* classes *)
+      -> list procedure (* procedures *)
+      -> library
+
+with class : Set :=
+  | Class : 
+      named_node_data
+      -> string (* name *)
+      -> list procedure (* procedures *)
+      -> class
+
+with member_data : Set :=
+  | Member : 
+      named_node_data
+      -> list expression (* annotations *)
+      -> name (* name *)
+      -> member_data
+
+with member : Set :=
+  | M_Procedure : procedure -> member
+
+
+with procedure : Set :=
+  | Procedure : 
+      member_data
+      -> named_node_data
+      -> function_node (* function *)
+      -> procedure
+
+with function_node : Set :=
+  | Function_Node : 
+      variable_declaration (* positionalParameters *)
+      -> dart_type (* returnType *)
+      -> statement (* body *)
+      -> function_node
+
+with expression : Set :=
+  | E_Variable_Get : variable_get -> expression
+  | E_Property_Get : property_get -> expression
+  | E_Invocation_Expression : invocation_expression -> expression
+
+
+with variable_get : Set :=
+  | Variable_Get : 
+      nat (* variable *)
+      -> variable_get
+
+with property_get : Set :=
+  | Property_Get : 
+      expression (* receiver *)
+      -> name (* name *)
+      -> property_get
+
+with arguments : Set :=
+  | Arguments : 
+      expression (* positional *)
+      -> arguments
+
+with invocation_expression : Set :=
+  | IE_Method_Invocation : method_invocation -> invocation_expression
+  | IE_Constructor_Invocation : constructor_invocation -> invocation_expression
+
+
+with method_invocation : Set :=
+  | Method_Invocation : 
+      expression (* receiver *)
+      -> name (* name *)
+      -> arguments (* arguments *)
+      -> nat (* interfaceTargetReference *)
+      -> method_invocation
+
+with constructor_invocation : Set :=
+  | Constructor_Invocation : 
+      nat (* targetReference *)
+      -> arguments (* arguments *)
+      -> constructor_invocation
+
+with statement : Set :=
+  | S_Expression_Statement : expression_statement -> statement
+  | S_Block : block -> statement
+  | S_Return_Statement : return_statement -> statement
+  | S_Variable_Declaration : variable_declaration -> statement
+
+
+with expression_statement : Set :=
+  | Expression_Statement : 
+      expression (* expression *)
+      -> expression_statement
+
+with block : Set :=
+  | Block : 
+      list statement (* statements *)
+      -> block
+
+with return_statement : Set :=
+  | Return_Statement : 
+      expression (* expression *)
+      -> return_statement
+
+with variable_declaration : Set :=
+  | Variable_Declaration : 
+      nat
+      -> dart_type (* type *)
+      -> option expression (* initializer *)
+      -> variable_declaration
+
+with name : Set :=
+  | Name : 
+      string (* name *)
+      -> name
+
+with dart_type : Set :=
+  | DT_Interface_Type : interface_type -> dart_type
+  | DT_Function_Type : function_type -> dart_type
+
+
+with interface_type : Set :=
+  | Interface_Type : 
+      nat (* className *)
+      -> interface_type
+
+with function_type : Set :=
+  | Function_Type : 
+      dart_type (* positionalParameters *)
+      -> dart_type (* returnType *)
+      -> function_type
+
+.
+
